Use faster `to_Z` function

rocq-bluerock-brick/theories/prelude/array_map.v
@@ -3,6 +3,473 @@ Require Import BinNatDef.
 Require Import Stdlib.Numbers.Cyclic.Int63.Uint63.
 Require Import bedrock.prelude.base.
 
+Module Uint63_Fast.
+
+    (* Faster than [to_Z], probably only for small-ish integers *)
+    Fixpoint to_Z_zero_rec (n : nat) (i : int) {struct n} : Z :=
+      if is_zero i then 0%Z else
+      match n with
+      | O => 0%Z
+      | S n0 => (if is_even i then Z.double else Z.succ_double) (to_Z_zero_rec n0 (i >> 1)%uint63)
+      end.
+    Definition to_Z_zero := to_Z_zero_rec Uint63.size.
+    Definition to_Z_zero' := Eval lazy [to_Z_zero_rec Uint63.size] in to_Z_zero_rec Uint63.size.
+
+
+    Definition to_Z_rec_shift (i : int) : Z :=
+      (fix go n k :=
+         match n with
+         | O => 0%Z
+         | S n0 => (if is_even (i >> k) then Z.double else Z.succ_double) (go n0 (k - 1)%uint63)
+         end) Uint63.size 62%uint63.
+    Definition to_Z_shift := to_Z_rec_shift.
+    Definition to_Z_shift' := Eval lazy [to_Z_rec_shift Uint63.size Uint63.sub] in to_Z_rec_shift.
+
+    Definition is_even_at (i : int) (bit : int) :=
+      (i land 1 << bit =? 0)%uint63.
+
+    Definition to_Z_rec_shift_at (i : int) : Z :=
+      (fix go n k :=
+         match n with
+         | O => 0%Z
+         | S n0 => (if is_even_at i (62-k) then Z.double else Z.succ_double) (go n0 (k - 1)%uint63)
+         end) Uint63.size 62%uint63.
+    Definition to_Z_shift_at := to_Z_rec_shift_at.
+    Definition to_Z_shift_at' := Eval lazy [to_Z_rec_shift_at Uint63.size Uint63.sub is_even_at Uint63.lsl] in to_Z_rec_shift_at.
+
+
+    Definition to_Z_rec_cps (i : int) : Z :=
+      (fix go n k cont :=
+         match n with
+         | O => cont 0%Z
+         | S n0 =>
+             go n0 (k + 1)%uint63 $ fun z =>
+             (if is_even_at i (62-k) then
+                Z.double
+              else
+                Z.succ_double) $ cont z
+         end) Uint63.size 0%uint63 (fun z => z).
+    Definition to_Z_cps := to_Z_rec_cps.
+    Definition to_Z_cps' := Eval lazy [to_Z_rec_cps Uint63.size Uint63.sub Uint63.add is_even_at Uint63.lsl] in to_Z_rec_cps.
+
+
+
+    (* highest bit in [0..62] *)
+    Definition zeros_below (i : int) (highest_bit : int) :=
+      (i land (max_int >> (63-highest_bit)) =? 0)%uint63.
+
+    Definition to_Z_rec_at_zero (i : int) : Z :=
+      (fix go n k :=
+         if zeros_below i k then 0%Z else
+         match n with
+         | O => 0%Z
+         | S n0 => (if is_even_at i (62-k) then Z.double else Z.succ_double) (go n0 (k - 1)%uint63)
+         end) Uint63.size 62%uint63.
+    Definition to_Z_at_zero := to_Z_rec_at_zero.
+    Definition to_Z_at_zero' :=
+      Eval lazy [
+          to_Z_rec_at_zero Uint63.size Uint63.sub is_even_at
+          Uint63.lsl Uint63.lsr
+          zeros_below
+          Uint63.max_int
+          opp
+        ] in to_Z_rec_at_zero.
+
+
+    Definition zeros_above (i : int) (highest_bit : int) :=
+      (i land (max_int << (highest_bit)) =? 0)%uint63.
+
+    (* Definition to_pos_rec (i : int) : positive := *)
+    (*   (fix go n k c := *)
+    (*      if zeros_above i (k+1) then c xH else *)
+    (*      match n with *)
+    (*      | O => c xH *)
+    (*      | S n0 => *)
+    (*          (go n0 (k + 1)%uint63) *)
+    (*            (fun p => c $ (if (is_even_at i k) then xO p else xI p)) *)
+    (*      end) Uint63.size 0%uint63 (fun x => x). *)
+
+    Definition to_pos_rec (i : int) : nat -> int -> positive :=
+      (fix go n k :=
+         match n with
+         | O => xH
+         | S n0 =>
+             if zeros_above i (k+1) then xH else
+             (if is_even_at i k then
+              xO
+             else
+              xI) $ go n0 (k + 1)%uint63
+         end).
+
+    Definition to_Z_pos (i : int) :=
+      if (i =? 0)%uint63 then 0%Z else Z.pos $ to_pos_rec i Uint63.size 0%uint63.
+
+    Require Import Stdlib.micromega.ZifyUint63.
+
+    Lemma decide_bounded (P : int -> Prop) `{P_dec : forall x, Decision (P x)} :
+      Decision (exists x, P x).
+    Proof.
+      suff: (Decision (exists x, x <=? max_int = true /\ P x)%uint63).
+      - move => [H|H]; [left|right].
+        + destruct H as [x [Hx H]].
+          exists x. auto.
+        + move => H'. apply: H. destruct H' as [x H]. exists x.
+          split; [lia|done].
+      - pose m := to_nat max_int.
+        have Hm : (m <= to_nat max_int)%nat by lia.
+        have ->: max_int = of_nat m by lia.
+        elim: m Hm => [|{}m IH] Hm.
+        + case: (P_dec 0%uint63) => [H0|H0].
+          * left. exists 0%uint63. split; [lia|done].
+          * right. move => [x [Hx HP]].
+            apply: H0.
+            by have ->: (0 = x)%uint63 by lia.
+        + case: (P_dec (of_nat (S m))) => [HPm|HPm].
+          * left. exists (of_nat (S m)). split; [lia|done].
+          * case: (IH ltac:(lia)) => [{}IH|{}IH].
+            { left. destruct IH as [x [IHx IH]]. exists x.
+              split; [lia|done]. }
+            { right. intros H. apply: IH. destruct H as [x [Hxm Hx]].
+              case H: (x =? of_nat (S m))%uint63.
+              { exfalso. apply HPm. by have ->: (of_nat (S m) = x) by lia. }
+              { exists x; split; [lia|done]. }
+            }
+    Qed.
+
+    Lemma brute_force P d :
+      nat_rect (fun i => Prop) (P 0) (fun n acc => P (S n) /\ acc) d ->
+      forall x, x <= d -> P x.
+    Proof.
+      induction d.
+      - simpl. move => H0 x Hx. by have ->: x = 0 by lia.
+      - simpl. move => [H1 H2] x Hx.
+        case Hx': (x =? S d)%nat.
+        { by have ->: x = S d by lia. }
+        apply IHd; [done|lia].
+    Qed.
+
+    Lemma bit_max_int b :
+      (b <? digits)%uint63 = true ->
+      bit max_int b = true.
+    Proof.
+      have ->: digits = of_nat 63 by lia.
+      move => H.
+      have Hb: b = of_nat (to_nat b) by lia.
+      have Hb': (to_nat b <= 63)%nat by lia.
+      move: H. rewrite {}Hb. move: (to_nat b) Hb' => {}b Hb Hb'.
+      refine (brute_force (fun x => bit max_int (of_nat x) = true) 62 _ _ _); [|lia].
+      vm_compute; by repeat split.
+    Qed.
+
+    Lemma zeros_above_false i j:
+      zeros_above i j = false <->
+      exists k, (to_Z j <= to_Z k < to_Z digits)%Z /\ bit i k = true.
+    Proof.
+      split.
+      - rewrite /zeros_above.
+        move/Uint63.eqb_false_spec.
+        simpl. rewrite -/max_int.
+        set P := (fun k => _ /\ _).
+        have ? : forall x, Decision (P x).
+        { intros. apply and_dec; apply _. }
+        case: (decide_bounded P).
+        { eauto. }
+        intros Hx Hi.
+        exfalso.
+        apply: Hi.
+        apply bit_ext => b.
+        rewrite land_spec bit_0.
+        case Hb: (digits <=? b)%uint63.
+        { by rewrite bit_M // andb_false_l bit_0. }
+        rewrite bit_lsl.
+        case_match; [lia|].
+        rewrite bit_max_int; [|lia].
+        rewrite andb_true_r.
+        have {}Hx: forall x, P x -> False.
+        { move => x Hx'. apply: Hx. eauto. }
+        specialize (Hx b). unfold P in Hx.
+        apply not_true_is_false => Hib.
+        apply: Hx.
+        split; [lia|done].
+      - move => [b [Hjb Hib]].
+        rewrite /zeros_above.
+        apply/Uint63.eqb_false_spec.
+        move/(f_equal (fun i => bit i b)).
+        rewrite land_spec.
+        case Hb: (digits <=? b)%uint63; [lia|].
+        rewrite bit_lsl.
+        case_match; [lia|].
+        rewrite bit_max_int; [|lia].
+        by rewrite andb_true_r Hib bit_0.
+    Qed.
+
+    Lemma bit_ext' (i j : int) :
+      (i =? j = true)%uint63 -> forall k, bit i k = bit j k.
+    Proof.
+      move/Uint63.eqb_spec => ->. done.
+    Qed.
+
+    Lemma zeros_above_true i j:
+      zeros_above i j = true ->
+      forall k, (j <=? k = true)%uint63 -> (k <? digits = true)%uint63 -> bit i k = false.
+    Proof.
+      rewrite /zeros_above.
+      move => /bit_ext' => H k Hjk Hkd.
+      rewrite -(bit_0 k).
+      specialize (H k%uint63).
+      move: H.
+      rewrite land_spec.
+      rewrite bit_lsl.
+      case H: (_ || _); [lia|].
+      apply orb_false_iff in H.
+      rewrite bit_max_int; [|lia].
+      by rewrite andb_true_r.
+    Qed.
+
+    Lemma zeros_above_true_2 i j:
+      (j <? digits = true)%uint63 ->
+      (forall k, (j <=? k = true)%uint63 -> (k <? digits = true)%uint63 -> bit i k = false) ->
+      zeros_above i j = true.
+    Proof.
+      move => H1 H2.
+      rewrite /zeros_above.
+      apply Uint63.eqb_spec. apply bit_ext => b.
+      rewrite bit_0.
+      rewrite land_spec.
+      rewrite bit_lsl.
+      case_match; [lia|].
+      rewrite bit_max_int; [|lia].
+      rewrite andb_true_r.
+      apply: H2; lia.
+    Qed.
+
+    Lemma zeros_above_true_shift i j:
+      zeros_above i j = true ->
+      (i >> j = 0)%uint63.
+    Proof.
+      move/zeros_above_true => H.
+      apply bit_ext => b.
+      rewrite bit_0.
+      rewrite bit_lsr.
+      case_match; [|reflexivity].
+      case Hb: (digits <=? j + b)%uint63.
+      { by rewrite bit_M. }
+      rewrite H; lia.
+    Qed.
+
+    Lemma bit_land_1_lsr i j:
+      (j <? digits)%uint63 = true ->
+      ((i >> j) land 1 =? 0)%uint63 = ~~ bit i j.
+    Proof.
+      pose k := to_nat j.
+      have ->: j = of_nat k by lia.
+      intros H.
+      have Hk: k < 63 by lia.
+      clear H.
+      move: {j} k Hk i.
+      elim => [|k IH] Hk i.
+      - simpl. rewrite lsr_0_r.
+        have := is_even_bit i.
+        by cbn => ->.
+      - intros.
+        have ->: (of_nat (S k) = of_nat k + 1)%uint63 by lia.
+        rewrite -bit_half; [|lia].
+        rewrite -IH; [|lia].
+        rewrite lsr_add.
+        case_match; [|lia].
+        f_equal.
+        f_equal.
+        f_equal.
+        lia.
+    Qed.
+
+    Lemma to_Z_rec_0 n : to_Z_rec n 0%uint63 = 0.
+    Proof.
+      induction n.
+      - done.
+      - cbn.
+        rewrite IHn.
+        lia.
+    Qed.
+
+    Lemma is_even_at_is_even i j:
+      (j <? digits = true)%uint63 ->
+      is_even_at i j = is_even (i >> j).
+    Proof.
+      intros.
+      rewrite /is_even_at/is_even/is_zero/=.
+      case Hea: (_ =? 0)%uint63 => //;
+      case He: (_ =? 0)%uint63 => //.
+      - rewrite bit_land_1_lsr in He; [|lia].
+        exfalso.
+        have {Hea} := (bit_ext' _ _ Hea j).
+        rewrite bit_0 -{}He.
+        rewrite land_spec.
+        rewrite bit_lsl.
+        case_match; [lia|].
+        have ->: (j - j = 0)%uint63 by lia.
+        rewrite andb_true_r. by case: (bit _ _).
+      - exfalso.
+        rewrite bit_land_1_lsr in He; [|lia].
+        apply Uint63.eqb_false_spec in Hea.
+        apply Hea.
+        apply bit_ext => b.
+        apply eq_sym in He.
+        apply negb_sym in He.
+        rewrite land_spec.
+        rewrite bit_lsl.
+        case_match.
+        { by rewrite andb_false_r bit_0. }
+        rewrite bit_1. case Hj: (_ =? 0)%uint63.
+        { have ->: (b = j) by lia. by rewrite He bit_0. }
+        { by rewrite andb_false_r bit_0. }
+    Qed.
+
+    Lemma to_Z_pos_rec_spec i :
+      to_Z_pos i = Uint63.to_Z i.
+    Proof.
+      unfold to_Z_pos.
+      case: (eqbP i 0)%uint63 => H.
+      { by have ->: (i = of_Z 0) by lia. }
+      unfold Uint63.to_Z.
+      set x := 0%uint63.
+      have : forall j, (0 <= to_Z j <= to_Z x)%Z -> zeros_above i j = false.
+      { intros. have ? : j = 0%uint63 by lia. subst.
+        rewrite /zeros_above lsl0_r.
+        apply eqb_false_spec.
+        move => Hi. 
+        apply H. rewrite -{}Hi.
+        f_equal.
+        apply bit_ext => b.
+        rewrite land_spec.
+        case Hb: (digits <=? b)%uint63.
+        { by rewrite !bit_M. }
+        rewrite bit_max_int; [|lia].
+        by rewrite andb_true_r.
+      }
+
+      have ->: x = (63 - of_nat (Uint63.size))%uint63 by done.
+      set j := {3}i.
+      have ->: j = (i >> (63 - of_nat (Uint63.size)))%uint63 by rewrite lsr_0_r.
+      set n := Uint63.size.
+      have Hn : n <= 63 by done.
+      clearbody n. clear x j.
+      induction n => Hz.
+      - cbn. simpl.
+        specialize (Hz 63%uint63 ltac:(lia)).
+        cbn in Hz.
+        rewrite land0_r in Hz. lia.
+      - unfold to_pos_rec.
+        case Hza: (zeros_above i (63 - of_nat (S n) + 1)).
+        + cbn.
+          have: bit i (63 - of_nat (S n)) = true.
+          { destruct (proj1 (zeros_above_false _ _) (Hz (63 - of_nat (S n))%uint63 ltac:(lia)))
+              as [b [Hb1 Hb2]].
+            case: (Uint63.eqbP b (63 - of_nat (S n)))%uint63 => Hb.
+            { move/(f_equal of_Z): Hb. rewrite !of_to_Z => ?. by subst. }
+            rewrite (zeros_above_true _ _ Hza b) in Hb2; [done|lia|lia].
+          }
+          rewrite bit_land_1_lsr; [|lia].
+          move => ->.
+          rewrite zeros_above_true_shift; [|].
+          { by rewrite to_Z_rec_0. }
+          apply zeros_above_true_2; [lia|].
+          intros.
+          rewrite bit_lsr.
+          case_match; [|lia].
+          case Ht: (digits <=? 63 - of_nat (S n) + k)%uint63.
+          { rewrite bit_M; [done|lia]. }
+          eapply zeros_above_true; [exact Hza|lia|lia].
+        + rewrite -/(to_pos_rec _).
+          case He: (is_even_at _ _).
+          * cbn -[is_even].
+            rewrite -is_even_at_is_even; [|lia].
+            rewrite He.
+            rewrite lsr_add.
+            case Hle: (_ <=? _)%uint63; [|lia].
+            move: Hza.
+            have ->: (63 - of_nat (S n) + 1 = 63 - of_nat n)%uint63 by lia.
+            move => Hza.
+            rewrite -{}IHn; [|lia|]; last first.
+            { move => j Hj.
+              case Hj': (j =? 63 - of_nat n)%uint63.
+              { apply Uint63.eqb_spec in Hj'. by subst. }
+              { apply Hz. lia. }
+            }
+            lia.
+          * cbn -[is_even].
+            rewrite -is_even_at_is_even; [|lia].
+            rewrite He.
+            rewrite lsr_add.
+            case Hle: (_ <=? _)%uint63; [|lia].
+            move: Hza.
+            have ->: (63 - of_nat (S n) + 1 = 63 - of_nat n)%uint63 by lia.
+            move => Hza.
+            rewrite -{}IHn; [|lia|]; last first.
+            { move => j Hj.
+              case Hj': (j =? 63 - of_nat n)%uint63.
+              { apply Uint63.eqb_spec in Hj'. by subst. }
+              { apply Hz. lia. }
+            }
+            lia.
+    Qed.
+
+
+    Definition to_Z_pos' :=
+      Eval lazy [
+          to_Z_pos
+          to_pos_rec
+          Uint63.size
+          Uint63.sub
+          Uint63.add
+          is_even_at
+          Uint63.lsl Uint63.lsr
+          zeros_above
+          Uint63.max_int
+          opp
+        ] in to_Z_pos.
+
+    Instructions Eval cbn in to_Z_pos' 1000.          (*   929641 *)
+    Instructions Eval cbn in to_Z_cps' 1000.          (*  1438046 *)
+    Instructions Eval cbn in to_Z_shift_at' 1000.     (*  1444908 *)
+    Instructions Eval cbn in to_Z_pos  1000.          (*  1580101 *)
+    Instructions Eval cbn in to_Z_at_zero' 1000.      (*  1927441 *)
+    Instructions Eval cbn in to_Z 1000.               (*  2658531 *)
+    Instructions Eval cbn in to_Z_shift' 1000.        (*  6758395 *)
+    Instructions Eval cbn in to_Z_shift_at 1000.      (* 11003813 *)
+    Instructions Eval cbn in to_Z_shift 1000.         (* 15617117 *)
+    Instructions Eval cbn in to_Z_at_zero 1000.       (* 17260218 *)
+    Instructions Eval cbn in Uint63.to_Z 1000.        (* 18665195 *)
+    Instructions Eval cbn in to_Z_cps 1000.           (* 42629956 *)
+
+    Instructions Eval cbn in to_Z_shift_at' max_int.  (*  6687966 *)
+    Instructions Eval cbn in to_Z_cps' max_int.       (*  6691650 *)
+    Instructions Eval cbn in to_Z_pos' max_int.       (*  6971998 *)
+    Instructions Eval cbn in to_Z_at_zero' max_int.   (*  7208922 *)
+    Instructions Eval cbn in to_Z_shift' max_int.     (*  7329249 *)
+    Instructions Eval cbn in to_Z_shift max_int.      (* 16188723 *)
+    Instructions Eval cbn in to_Z_shift_at max_int.   (* 16248515 *)
+    Instructions Eval cbn in to_Z_pos max_int.        (* 23770184 *)
+    Instructions Eval cbn in Uint63.to_Z max_int.     (* 23912206 *)
+    Instructions Eval cbn in to_Z_at_zero max_int.    (* 23994139 *)
+    Instructions Eval cbn in to_Z max_int.            (* 34248352 *)
+    Instructions Eval cbn in to_Z_cps max_int.        (* 47883930 *)
+
+
+    Instructions Eval lazy in to_Z_shift_at' max_int. (*  5952206 *)
+    Instructions Eval lazy in to_Z_cps' max_int.      (*  5956495 *)
+    Instructions Eval lazy in to_Z_at_zero' max_int.  (*  6067052 *)
+    Instructions Eval lazy in to_Z_pos' max_int.      (*  6091810 *)
+    Instructions Eval lazy in to_Z_shift' max_int.    (*  6151919 *)
+    Instructions Eval lazy in Uint63.to_Z max_int.    (*  6359392 *)
+    Instructions Eval lazy in to_Z_shift max_int.     (*  6492338 *)
+    Instructions Eval lazy in to_Z max_int.           (*  6565755 *)
+    Instructions Eval lazy in to_Z_cps max_int.       (*  6643789 *)
+    Instructions Eval lazy in to_Z_shift_at max_int.  (*  6799749 *)
+    Instructions Eval lazy in to_Z_pos max_int.       (*  6902058 *)
+    Instructions Eval lazy in to_Z_at_zero max_int.   (*  6990130 *)
+
+End Uint63_Fast.
 Module Type KEY.
   Parameter key : Type.
   Declare Instance inh : Inhabited key.
@@ -105,7 +572,7 @@ Module map (Import K : KEY).
 
     Definition find_key (needle : key) (m : t) : option idx :=
       Eval lazy match iota beta delta [Z.to_N] in
-      let len := Z.to_N (to_Z (PArray.length m.(keys))) in
+      let len := Z.to_N (Uint63_Fast.to_Z_pos (PArray.length m.(keys))) in
       binary_search m.(keys) needle $ bisect_N len.
 
     Definition find (needle : key) (m : t) : option elt :=
@@ -164,7 +631,7 @@ Module map (Import K : KEY).
       end.
 
     Definition fold {A} (f : key -> elt -> A -> A) (m : t) (acc : A) : A :=
-      fold_to f m (Z.to_nat $ to_Z $ PArray.length m.(keys)) 0 acc.
+      fold_to f m (Z.to_nat $ Uint63_Fast.to_Z_pos $ PArray.length m.(keys)) 0 acc.
 
     #[local]
     Fixpoint elements_to (m : t) (count : nat) (i : int) (acc : list (key * elt)) : list (key * elt) :=
@@ -174,7 +641,7 @@ Module map (Import K : KEY).
       end.
 
     Definition elements (m : t) : list (key * elt) :=
-      elements_to m (Z.to_nat $ to_Z $ PArray.length m.(keys)) (PArray.length m.(keys) - 1)%uint63 nil.
+      elements_to m (Z.to_nat $ Uint63_Fast.to_Z_pos $ PArray.length m.(keys)) (PArray.length m.(keys) - 1)%uint63 nil.
 
     #[local]
     Fixpoint find_any_to (f : key -> elt -> bool) (m : t) (count : nat) (i : int) : bool :=
@@ -186,19 +653,20 @@ Module map (Import K : KEY).
       end.
 
     Definition find_any (f : key -> elt -> bool) (m : t) :=
-      find_any_to f m (Z.to_nat $ to_Z $ PArray.length m.(keys)) (PArray.length m.(keys) - 1)%uint63.
+      find_any_to f m (Z.to_nat $ Uint63_Fast.to_Z_pos $ PArray.length m.(keys)) (PArray.length m.(keys) - 1)%uint63.
 
     Definition copy (m : t) : t :=
       mk (PArray.copy m.(keys)) (PArray.copy m.(values)).
 
     Definition cardinal (m : t) : nat :=
-      Z.to_nat $ to_Z $ PArray.length m.(keys).
+      Z.to_nat $ Uint63_Fast.to_Z_pos $ PArray.length m.(keys).
 
     Lemma cardinal_1 : forall m, cardinal m = length (elements m).
     Proof.
       rewrite /cardinal/elements.
       intros.
       move L: (PArray.length (keys m)) => len.
+      rewrite Uint63_Fast.to_Z_pos_rec_spec.
       move : (to_nat len) => n.
       have {1}-> : n = n + @length (key * elt) [] by done.
       move: (len - 1)%uint63 => i.
